src/Bisimulations.v
@@ -12,24 +12,28 @@ Proof.
   {
     subst. induction H0.
     * eexists. split. 2: reflexivity.
-      eapply nsend; try eassumption.
+      eapply n_send; try eassumption.
     * eexists. split. 2: reflexivity.
-      eapply narrive; try eassumption.
+      eapply n_arrive; try eassumption.
     * eexists. split. 2: reflexivity.
-      eapply nother; try eassumption.
+      eapply n_other; try eassumption.
     * eexists. split. 2: reflexivity.
-      eapply nspawn; try eassumption.
+      eapply n_spawn; try eassumption.
+    * eexists. split. 2: reflexivity.
+      eapply n_terminate. auto.
   }
   {
     subst. induction H0.
     * eexists. split. 2: reflexivity.
-      eapply nsend; try eassumption.
+      eapply n_send; try eassumption.
     * eexists. split. 2: reflexivity.
-      eapply narrive; try eassumption.
+      eapply n_arrive; try eassumption.
     * eexists. split. 2: reflexivity.
-      eapply nother; try eassumption.
+      eapply n_other; try eassumption.
     * eexists. split. 2: reflexivity.
-      eapply nspawn; try eassumption.
+      eapply n_spawn; try eassumption.
+    * eexists. split. 2: reflexivity.
+      eapply n_terminate. auto.
   }
 Qed.
 
@@ -108,7 +112,7 @@ pidCompatibleNode A A' /\ .
 
 
 Definition internals (n n' : Node) : Prop :=
-  exists l k, Forall (fun e => fst e = AInternal) l /\ n -[k|l]ₙ->* n'.
+  exists l k, Forall (fun e => e.1 = AInternal) l /\ n -[k|l]ₙ->* n'.
 
 Notation "n -->* n'" := (internals n n') (at level 50).
 
@@ -158,37 +162,11 @@ Proof.
   * inversion H1. subst. rewrite H in H7. now inversion H7.
 Qed.
 
-(* Lemma internal_alt : forall ether ether' procs procs' a ι p,
-  (ether, procs) -[ a | ι ]ₙ-> (ether', procs') -> Some p = proc' ι -> Π -[ a | ι ]ₙ-> ι : p |||| Π'.
-Proof.
-  intros. generalize dependent p. induction H; intros; try rewrite par_same.
-  * unfold par in H2; break_match_hyp. 2: congruence. inversion H2. subst. now apply nsend1.
-  * unfold par in H1; break_match_hyp. 2: congruence. inversion H1. subst. eapply nsend2; eauto.
-  * unfold par in H1; break_match_hyp. 2: congruence. inversion H1. subst. apply nsend3; eauto.
-  * unfold par in H0; break_match_hyp. 2: congruence. inversion H0. subst. constructor; eauto.
-  * unfold par in H0; break_match_hyp. 2: congruence. inversion H0. subst. constructor; eauto.
-  * unfold par in H0; break_match_hyp. 2: congruence. inversion H0. subst. constructor; eauto.
-  * unfold par in H2; break_match_hyp.
-    - subst. unfold par in H0; break_match_hyp; congruence.
-    - break_match_hyp. 2: congruence. inversion H2. subst. 
-      rewrite par_swap, par_same. constructor; eauto. auto.
-Qed. *)
-
-Definition actionPid (a : Action) : option PID :=
-match a with
- | ASend p t => Some p
- | AReceive t => None
- | AArrive t => None
- | ASelf ι => None
- | ASpawn ι t1 t2 => Some ι
- | AInternal => None
-end.
-
 Lemma par_eq : forall ι p p' Π Π',
   ι : p |||| Π = ι : p' |||| Π' -> p = p'.
 Proof.
   intros. apply equal_f with ι in H as H'.
-  unfold par in H'; break_match_hyp. 2: congruence. inversion H'. auto.
+  unfold par, update in H'; break_match_hyp. 2: congruence. inversion H'. auto.
 Qed.
 
 Lemma concurrent_determinism :
@@ -198,13 +176,13 @@ Proof.
   * inversion H4; subst.
     - apply par_eq in H2 as H2'. subst.
       eapply internal_determinism in H. 2:exact H7. subst. auto. f_equal.
-      extensionality ι''. apply equal_f with ι'' in H2. unfold par in *.
+      extensionality ι''. apply equal_f with ι'' in H2. unfold par, update in *.
       break_match_goal; auto.
     - intuition; try congruence. destruct H3. congruence.
   * inversion H5; subst.
     - apply par_eq in H2 as H2'. inversion H2'. subst.
       eapply internal_determinism in H0. 2: exact H8. subst.
-      f_equal. extensionality ι''. apply equal_f with ι'' in H2. unfold par in *.
+      f_equal. extensionality ι''. apply equal_f with ι'' in H2. unfold par, update in *.
       break_match_goal; auto.
     - intuition; try congruence. destruct H4. congruence.
   * inversion H5; subst.
@@ -212,23 +190,30 @@ Proof.
     - intuition; try congruence. destruct H0. congruence.
     - apply par_eq in H2 as H2'. subst.
       eapply internal_determinism in H. 2: exact H3. subst. f_equal.
-      extensionality ι''. apply equal_f with ι'' in H2. unfold par in *.
+      extensionality ι''. apply equal_f with ι'' in H2. unfold par, update in *.
       break_match_goal; auto.
     - intuition; try congruence. destruct H0. congruence.
+    - apply par_eq in H3 as H3'. subst.
+      inversion H; subst; try inversion_is_value.
   * inversion H6; subst.
     - intuition; try congruence. destruct H5. congruence.
     - apply par_eq in H3 as H3'. subst.
       eapply internal_determinism in H1. 2: exact H12. subst.
       f_equal. rewrite H in H10. inversion H10. subst.
-      extensionality ι''. apply equal_f with ι'' in H3. unfold par in *.
+      extensionality ι''. apply equal_f with ι'' in H3. unfold par, update in *.
       break_match_goal; auto.
       break_match_goal; auto.
+  * inversion H4; subst.
+    - apply par_eq in H1 as H1'. subst.
+      inversion H2; subst; try inversion_is_value.
+    - unfold par, update in *. f_equal.
+      extensionality ι'. apply equal_f with ι' in H2. break_match_goal; auto.
 Qed.
 
 Lemma internal_equal :
   forall p p', p -⌈ AInternal ⌉-> p' -> forall p'' a, p -⌈ a ⌉-> p''
 ->
-  (a = AInternal /\ p'' = p') \/ (exists t, a = AArrive t /\ p'' = (fst (fst p), snd (fst p), snd p ++ [t])).
+  (a = AInternal /\ p'' = p') \/ (exists t, a = AArrive t /\ p'' = (p.1.1, p.1.2, p.2 ++ [t])).
 Proof.
   intros. inversion H; subst; inversion H0; subst.
   all: try (inversion H1; subst; inversion_is_value); auto; try inversion_is_value.
@@ -261,7 +246,7 @@ Lemma internal_det :
                                  exists n''', n' -[AArrive t | ι]ₙ-> n''' /\
                                  n''' = modifyMailbox ι ι t n').
 Proof.
-  intros. inversion H. inversion H0; subst.
+  intros. inversion H; inversion H0; subst.
   * inversion H8; subst. apply par_eq in H5. subst.
     eapply internal_equal in H7; eauto. destruct H7 as [[? ?] | [? [? ?]]]; congruence.
   * right. inversion H9; subst. apply par_eq in H5; subst.
@@ -270,23 +255,25 @@ Proof.
     destruct p,p. simpl in H4. subst. exists t.
     split; auto. split.
     - simpl. f_equal.
-      unfold par. inversion H3. subst.
+      unfold par, update. inversion H3. subst.
       extensionality ι'.
       break_match_goal; auto.
     - simpl. inversion H3. subst.
-      exists (etherPop (ι, x) ether, ι : (fst (fst p'), snd (fst p'), snd p' ++ [x]) |||| Π).
+      exists (etherPop (ι, x) ether, ι : (p'.1.1, p'.1.2, p'.2 ++ [x]) |||| Π).
       split.
-      + apply narrive; auto. destruct p', p. simpl. apply p_arrive; auto.
+      + apply n_arrive; auto. destruct p', p. simpl. apply p_arrive; auto.
         inversion H8; auto.
-      + f_equal. extensionality ι'. unfold par. break_match_goal; simpl.
+      + f_equal. extensionality ι'. unfold par, update. break_match_goal; simpl.
         destruct p',p. auto. auto.
   * inversion H9; subst. apply par_eq in H5; subst.
     eapply internal_equal in H7. 2: exact H1. destruct H7 as [[? ?] | [? [? ?]]]; try congruence.
     - subst. left; split; auto. f_equal. inversion H9.
-      extensionality x. apply equal_f with x in H4. unfold par in *. break_match_goal; auto.
+      extensionality x. apply equal_f with x in H4. unfold par, update in *. break_match_goal; auto.
     - subst. inversion H8. 2: inversion H3. 3: destruct H4. all: try congruence.
   * inversion H10; subst. apply par_eq in H5. subst.
     eapply internal_equal in H9; eauto. destruct H9 as [[? ?] | [? [? ?]]]; congruence.
+  * inversion H8; subst. apply par_eq in H5. subst.
+    inversion H1; subst; try inversion_is_value. now apply value_nostep in H9.
 Qed.
 
 Definition bothSpawn (a1 a2 : Action) : Prop:=
@@ -306,7 +293,7 @@ Proof.
   * inversion H4; subst.
     - exists ((ether ++ [(ι', t)]) ++ [(ι'1, t0)], ι'0 : p'0 |||| ι : p' |||| prs ).
       replace (ι : p' |||| prs) with (ι'0 : p0 |||| ι : p' |||| prs) at 1.
-      2: { extensionality ι1. unfold par in *. apply equal_f with ι1 in H2.
+      2: { extensionality ι1. unfold par, update in *. apply equal_f with ι1 in H2.
            break_match_goal; subst.
            break_match_goal; subst. congruence. auto.
            auto.
@@ -315,7 +302,7 @@ Proof.
     - exists (etherPop (ι'0, t0) (ether ++ [(ι', t)])
               , ι'0 : p'0 |||| ι : p' |||| prs ).
       replace (ι : p' |||| prs) with (ι'0 : p0 |||| ι : p' |||| prs) at 1.
-      2: { extensionality ι1. unfold par in *. apply equal_f with ι1 in H1.
+      2: { extensionality ι1. unfold par, update in *. apply equal_f with ι1 in H1.
            break_match_goal; subst.
            break_match_goal; subst. congruence. auto.
            auto.
@@ -324,7 +311,7 @@ Proof.
       apply in_or_app. now left.
     - exists (ether ++ [(ι', t)], ι'0 : p'0 |||| ι : p' |||| prs).
       replace (ι : p' |||| prs) with (ι'0 : p0 |||| ι : p' |||| prs) at 1.
-      2: { extensionality ι1. unfold par in *. apply equal_f with ι1 in H1.
+      2: { extensionality ι1. unfold par, update in *. apply equal_f with ι1 in H1.
            break_match_goal; subst.
            break_match_goal; subst. congruence. auto.
            auto.
@@ -333,21 +320,30 @@ Proof.
     - exists (ether ++ [(ι', t)], 
               ι'1 : ([], EApp v1 l, []) |||| ι'0 : p'0 |||| ι : p' |||| prs).
       replace (ι : p' |||| prs) with (ι'0 : p0 |||| ι : p' |||| prs) at 1.
-      2: { extensionality ι1. unfold par in *. apply equal_f with ι1 in H1.
+      2: { extensionality ι1. unfold par, update in *. apply equal_f with ι1 in H1.
            break_match_goal; subst.
            break_match_goal; subst. congruence. auto.
            auto.
          }
       constructor; auto.
       apply equal_f with ι'1 in H1.
-      unfold par in *. break_match_goal; auto.
+      unfold par, update in *. break_match_goal; auto.
       break_match_goal; subst.
       + congruence.
       + now rewrite H1 in H3.
+    - exists (ether ++ [(ι', t)],
+               ι : p' |||| prs -- ι'0).
+      replace (ι : p' |||| prs) with (ι'0 : ([], v, mb) |||| ι : p' |||| prs) at 1.
+      2: { extensionality ι1. unfold par, update in *. apply equal_f with ι1 in H2.
+           break_match_goal; subst.
+           break_match_goal; subst. congruence. auto.
+           auto.
+         }
+      constructor; auto.
   * inversion H5; subst.
     - exists (etherPop (ι, t) ether ++ [(ι'0, t0)], ι' : p'0 |||| ι : p' |||| prs).
       replace (ι : p' |||| prs) with (ι' : p0 |||| ι : p' |||| prs) at 1.
-      2: { extensionality ι1. unfold par in *. apply equal_f with ι1 in H3.
+      2: { extensionality ι1. unfold par, update in *. apply equal_f with ι1 in H3.
            break_match_goal; subst.
            break_match_goal; subst. congruence. auto.
            auto.
@@ -356,7 +352,7 @@ Proof.
     - exists (etherPop (ι', t0) (etherPop (ι, t) ether)
               , ι' : p'0 |||| ι : p' |||| prs ).
       replace (ι : p' |||| prs) with (ι' : p0 |||| ι : p' |||| prs) at 1.
-      2: { extensionality ι1. unfold par in *. apply equal_f with ι1 in H2.
+      2: { extensionality ι1. unfold par, update in *. apply equal_f with ι1 in H2.
            break_match_goal; subst.
            break_match_goal; subst. congruence. auto.
            auto.
@@ -365,7 +361,7 @@ Proof.
       apply removeFirst_In; auto. intro. apply H6. now inversion H1.
     - exists ((etherPop (ι, t) ether), ι' : p'0 |||| ι : p' |||| prs).
       replace (ι : p' |||| prs) with (ι' : p0 |||| ι : p' |||| prs) at 1.
-      2: { extensionality ι1. unfold par in *. apply equal_f with ι1 in H2.
+      2: { extensionality ι1. unfold par, update in *. apply equal_f with ι1 in H2.
            break_match_goal; subst.
            break_match_goal; subst. congruence. auto.
            auto.
@@ -374,21 +370,30 @@ Proof.
     - exists ((etherPop (ι, t) ether), 
               ι'0 : ([], EApp v1 l, []) |||| ι' : p'0 |||| ι : p' |||| prs).
       replace (ι : p' |||| prs) with (ι' : p0 |||| ι : p' |||| prs) at 1.
-      2: { extensionality ι1. unfold par in *. apply equal_f with ι1 in H2.
+      2: { extensionality ι1. unfold par, update in *. apply equal_f with ι1 in H2.
            break_match_goal; subst.
            break_match_goal; subst. congruence. auto.
            auto.
          }
       constructor; auto.
       apply equal_f with ι'0 in H2.
-      unfold par in *. break_match_goal; auto.
+      unfold par, update in *. break_match_goal; auto.
       break_match_goal; subst.
       + congruence.
       + now rewrite H2 in H4.
+    - exists (etherPop (ι, t) ether,
+               ι : p' |||| prs -- ι').
+      replace (ι : p' |||| prs) with (ι' : ([], v, mb) |||| ι : p' |||| prs) at 1.
+      2: { extensionality ι1. unfold par, update in *. apply equal_f with ι1 in H3.
+           break_match_goal; subst.
+           break_match_goal; subst. congruence. auto.
+           auto.
+         }
+      constructor; auto.
   * inversion H5; subst.
     - exists (ether ++ [(ι'0, t)], ι' : p'0 |||| ι : p' |||| Π).
       replace (ι : p' |||| Π) with (ι' : p0 |||| ι : p' |||| Π) at 1.
-      2: { extensionality ι1. unfold par in *. apply equal_f with ι1 in H3.
+      2: { extensionality ι1. unfold par, update in *. apply equal_f with ι1 in H3.
            break_match_goal; subst.
            break_match_goal; subst. congruence. auto.
            auto.
@@ -397,7 +402,7 @@ Proof.
     - exists (etherPop (ι', t) ether
               , ι' : p'0 |||| ι : p' |||| Π ).
       replace (ι : p' |||| Π) with (ι' : p0 |||| ι : p' |||| Π) at 1.
-      2: { extensionality ι1. unfold par in *. apply equal_f with ι1 in H2.
+      2: { extensionality ι1. unfold par, update in *. apply equal_f with ι1 in H2.
            break_match_goal; subst.
            break_match_goal; subst. congruence. auto.
            auto.
@@ -405,7 +410,7 @@ Proof.
       constructor; auto.
     - exists (ether, ι' : p'0 |||| ι : p' |||| Π).
       replace (ι : p' |||| Π) with (ι' : p0 |||| ι : p' |||| Π) at 1.
-      2: { extensionality ι1. unfold par in *. apply equal_f with ι1 in H2.
+      2: { extensionality ι1. unfold par, update in *. apply equal_f with ι1 in H2.
            break_match_goal; subst.
            break_match_goal; subst. congruence. auto.
            auto.
@@ -414,22 +419,31 @@ Proof.
     - exists (ether, 
               ι'0 : ([], EApp v1 l, []) |||| ι' : p'0 |||| ι : p' |||| Π).
       replace (ι : p' |||| Π) with (ι' : p0 |||| ι : p' |||| Π) at 1.
-      2: { extensionality ι1. unfold par in *. apply equal_f with ι1 in H2.
+      2: { extensionality ι1. unfold par, update in *. apply equal_f with ι1 in H2.
            break_match_goal; subst.
            break_match_goal; subst. congruence. auto.
            auto.
          }
       constructor; auto.
       apply equal_f with ι'0 in H2.
-      unfold par in *. break_match_goal; auto.
+      unfold par, update in *. break_match_goal; auto.
       break_match_goal; subst.
       + congruence.
       + now rewrite H2 in H4.
+    - exists (ether,
+               ι : p' |||| Π -- ι').
+      replace (ι : p' |||| Π) with (ι' : ([], v, mb) |||| ι : p' |||| Π) at 1.
+      2: { extensionality ι1. unfold par, update in *. apply equal_f with ι1 in H3.
+           break_match_goal; subst.
+           break_match_goal; subst. congruence. auto.
+           auto.
+         }
+      constructor; auto.
   * inversion H6; subst.
     - exists (ether ++ [(ι'1, t)], ι'0 : p'0 |||| ι' : ([], EApp v1 l, []) |||| ι : p' |||| Π).
       replace (ι' : ([], EApp v1 l, []) |||| ι : p' |||| Π) with 
               (ι'0 : p0 |||| ι' : ([], EApp v1 l, []) |||| ι : p' |||| Π) at 1.
-      2: { extensionality ι1. unfold par in *. apply equal_f with ι1 in H4.
+      2: { extensionality ι1. unfold par, update in *. apply equal_f with ι1 in H4.
            break_match_goal; subst;
            break_match_goal; subst; auto.
            all: break_match_hyp; auto; congruence.
@@ -439,7 +453,7 @@ Proof.
               , ι'0 : p'0 |||| ι' : ([], EApp v1 l, []) |||| ι : p' |||| Π ).
       replace (ι' : ([], EApp v1 l, []) |||| ι : p' |||| Π) with 
               (ι'0 : p0 |||| ι' : ([], EApp v1 l, []) |||| ι : p' |||| Π) at 1.
-      2: { extensionality ι1. unfold par in *. apply equal_f with ι1 in H3.
+      2: { extensionality ι1. unfold par, update in *. apply equal_f with ι1 in H3.
            break_match_goal; subst;
            break_match_goal; subst; auto.
            all: break_match_hyp; auto; try congruence.
@@ -448,7 +462,7 @@ Proof.
     - exists (ether, ι'0 : p'0 |||| ι' : ([], EApp v1 l, []) |||| ι : p' |||| Π).
       replace (ι' : ([], EApp v1 l, []) |||| ι : p' |||| Π) with 
               (ι'0 : p0 |||| ι' : ([], EApp v1 l, []) |||| ι : p' |||| Π) at 1.
-      2: { extensionality ι1. unfold par in *. apply equal_f with ι1 in H3.
+      2: { extensionality ι1. unfold par, update in *. apply equal_f with ι1 in H3.
            break_match_goal; subst;
            break_match_goal; subst; auto.
            all: break_match_hyp; auto; congruence.
@@ -456,10 +470,67 @@ Proof.
       now constructor.
     - (** cannot be sure to generate different spawn PID-s *)
       exfalso. apply Spawns. cbn. auto.
+    - exists (ether,
+               ι' : ([], EApp v1 l, []) |||| ι : p' |||| Π -- ι'0).
+      replace (ι' : ([], EApp v1 l, []) |||| ι : p' |||| Π) with 
+              (ι'0 : ([], v, mb) |||| ι' : ([], EApp v1 l, []) |||| ι : p' |||| Π) at 1.
+      2: { extensionality ι1. unfold par, update in *. apply equal_f with ι1 in H4.
+           break_match_goal; subst.
+           break_match_goal; subst. congruence.
+           break_match_goal; auto. congruence.
+           break_match_goal; auto.
+         }
+      constructor; auto.
+  * inversion H4; subst.
+    - exists (ether ++ [(ι'0, t)], ι' : p' |||| (Π -- ι)).
+      replace (Π -- ι) with (ι' : p |||| (Π -- ι)) at 1.
+      2: { extensionality ι1. unfold par, update in *. apply equal_f with ι1 in H2.
+           break_match_goal; subst.
+           break_match_goal; subst. congruence. auto.
+           auto.
+         }
+      now constructor.
+    - exists (etherPop (ι', t) ether
+              , ι' : p' |||| (Π -- ι) ).
+      replace (Π -- ι) with (ι' : p |||| (Π -- ι)) at 1.
+      2: { extensionality ι1. unfold par, update in *. apply equal_f with ι1 in H1.
+           break_match_goal; subst.
+           break_match_goal; subst. congruence. auto.
+           auto.
+         }
+      constructor; auto.
+    - exists (ether, ι' : p' |||| (Π -- ι)).
+      replace (Π -- ι) with (ι' : p |||| (Π -- ι)) at 1.
+      2: { extensionality ι1. unfold par, update in *. apply equal_f with ι1 in H1.
+           break_match_goal; subst.
+           break_match_goal; subst. congruence. auto.
+           auto.
+         }
+      now constructor.
+    - exists (ether, 
+              ι'0 : ([], EApp v1 l, []) |||| ι' : p' |||| (Π -- ι)).
+      replace (Π -- ι) with (ι' : p |||| (Π -- ι)) at 1.
+      2: { extensionality ι1. unfold par, update in *. apply equal_f with ι1 in H1.
+           break_match_goal; subst.
+           break_match_goal; subst. congruence. auto.
+           auto.
+         }
+      constructor; auto.
+      apply equal_f with ι'0 in H1.
+      unfold par, update in *. break_match_goal; auto.
+      break_match_goal; subst; auto. congruence.
+    - exists (ether, (Π -- ι) -- ι').
+      replace (Π -- ι) with (ι' : ([], v0, mb0) |||| (Π -- ι)) at 1.
+      2: { extensionality ι1. unfold par, update in *. apply equal_f with ι1 in H2.
+           break_match_goal; subst. auto.
+           break_match_goal; subst. congruence. auto.
+           break_match_goal; subst; auto.
+         }
+      constructor; auto.
 Qed.
 
 Corollary chain_to_end :
-  forall n n' l k, n -[k | l]ₙ->* n' -> Forall (fun a => fst a = AInternal) l -> 
+  forall n n' l k, n -[k | l]ₙ->* n' -> Forall (fun a => a.1 = AInternal) l -> 
    forall n'' a ι, n -[a | ι]ₙ-> n''
 ->
   (exists n3 n4 l1 l2 k1 k2, a = AInternal /\ 
@@ -491,7 +562,7 @@ Proof.
       + left. destruct H2 as [k2 [eq1 [D1 [D2 [ D3 [eq2 eq3]]]]]]. subst.
         exists n3, n4, ((AInternal, ι)::l1), l2, (S k1), k2. split; auto.
         split. 2: split. 3: split. all: auto.
-        eapply ntrans. 2: exact D1. auto.
+        eapply n_trans. 2: exact D1. auto.
       + right. now exists t.
 Qed.
 
@@ -501,7 +572,7 @@ Lemma internal_keep :
   forall x, x <> ι -> snd n x = snd n' x.
 Proof.
   intros. inversion H; subst.
-  simpl. unfold par. break_match_goal; auto. congruence.
+  simpl. unfold par, update. break_match_goal; auto. congruence.
 Qed.
 
 (* general case wont work: message ordering is desructed *)
@@ -518,20 +589,20 @@ Proof.
     2: { intuition; try congruence. destruct H5; congruence. }
     assert (p = p0). {
       apply internal_keep with (x := ι2) in H0. simpl in H0.
-      unfold par in H0. break_match_hyp. now inversion H0. congruence.
+      unfold par, update in H0. break_match_hyp. now inversion H0. congruence.
       auto.
     }
     subst.
     subst. eapply internal_determinism in H3. 2: exact H9. subst.
     assert ((ι1 : p1 |||| ι2 : p' |||| prs0) = ι1 : p1 |||| ι2 : p' |||| prs) as EQ. {
-      extensionality x. unfold par in *. break_match_goal; auto.
+      extensionality x. unfold par, update in *. break_match_goal; auto.
       apply internal_keep with (x := x) in H0. simpl in H0.
       break_match_goal; auto. auto.
     }
     replace (ι2 : p' |||| prs0) with (ι1 : p1 |||| ι2 : p' |||| prs0).
     replace (ι2 : p' |||| prs) with (ι1 : p'1 |||| ι2 : p' |||| prs).
     rewrite EQ. constructor; auto.
-    all: unfold par in *; extensionality x; 
+    all: unfold par, update in *; extensionality x; 
          apply equal_f with x in H5; apply equal_f with x in H11;
          do 2 break_match_goal; subst; auto; congruence.
   * inversion H1; subst.
@@ -539,41 +610,41 @@ Proof.
     2: { intuition; try congruence. destruct H6; congruence. }
     assert (p = p0). {
       apply internal_keep with (x := ι2) in H0. simpl in H0.
-      unfold par in H0. break_match_hyp. now inversion H0. congruence.
+      unfold par, update in H0. break_match_hyp. now inversion H0. congruence.
       auto.
     }
     subst.
     subst. eapply internal_determinism in H4. 2: exact H8. subst.
     assert ((ι1 : p1 |||| ι2 : p' |||| prs0) = ι1 : p1 |||| ι2 : p' |||| prs) as EQ. {
-      extensionality x. unfold par in *. break_match_goal; auto.
+      extensionality x. unfold par, update in *. break_match_goal; auto.
       apply internal_keep with (x := x) in H0. simpl in H0.
       break_match_goal; auto. auto.
     }
     replace (ι2 : p' |||| prs0) with (ι1 : p1 |||| ι2 : p' |||| prs0).
     replace (ι2 : p' |||| prs) with (ι1 : p'1 |||| ι2 : p' |||| prs).
     rewrite EQ. constructor; auto.
-    all: unfold par in *; extensionality x; 
+    all: unfold par, update in *; extensionality x; 
          apply equal_f with x in H7; apply equal_f with x in H13;
          do 2 break_match_goal; subst; auto; congruence.
   * inversion H1; subst.
-    1,2,4: intuition; try congruence; destruct H4; congruence.
+    1,2,4,5: intuition; try congruence; destruct H4; congruence.
     inversion H0; subst.
     assert (p = p0). {
       apply internal_keep with (x := ι2) in H0. simpl in H0.
-      unfold par in H0. break_match_hyp. now inversion H0. congruence.
+      unfold par, update in H0. break_match_hyp. now inversion H0. congruence.
       auto.
     }
     subst.
     subst. eapply internal_determinism in H3. 2: exact H5. subst.
     assert ((ι1 : p1 |||| ι2 : p' |||| Π0) = ι1 : p1 |||| ι2 : p' |||| Π) as EQ. {
-      extensionality x. unfold par in *. break_match_goal; auto.
+      extensionality x. unfold par, update in *. break_match_goal; auto.
       apply internal_keep with (x := x) in H0. simpl in H0.
       break_match_goal; auto. auto.
     }
     replace (ι2 : p' |||| Π0) with (ι1 : p1 |||| ι2 : p' |||| Π0).
     replace (ι2 : p' |||| Π) with (ι1 : p'1 |||| ι2 : p' |||| Π).
     rewrite EQ. constructor; auto.
-    all: unfold par in *; extensionality x; 
+    1-2: unfold par, update in *; extensionality x; 
          apply equal_f with x in H8; apply equal_f with x in H13;
          do 2 break_match_goal; subst; auto; congruence.
   * inversion H1; subst.
@@ -581,14 +652,14 @@ Proof.
     inversion H0; subst.
     assert (p = p0). {
       apply internal_keep with (x := ι2) in H0. simpl in H0.
-      unfold par in H0. break_match_hyp. now inversion H0. congruence.
+      unfold par, update in H0. break_match_hyp. now inversion H0. congruence.
       auto.
     }
     subst.
     subst. eapply internal_determinism in H5. 2: exact H14. subst.
     assert ((ι1 : p1 |||| ι' : ([], EApp v1 l0, []) |||| ι2 : p' |||| Π0) = 
              ι1 : p1 |||| ι' : ([], EApp v1 l0, []) |||| ι2 : p' |||| Π) as EQ. {
-      extensionality x. unfold par in *. break_match_goal; auto.
+      extensionality x. unfold par, update in *. break_match_goal; auto.
       break_match_goal; auto.
       apply internal_keep with (x := x) in H0. simpl in H0.
       break_match_goal; auto.
@@ -599,13 +670,30 @@ Proof.
             (ι1 : p1 |||| ι' : ([], EApp v1 l0, []) |||| ι2 : p' |||| Π0).
     replace (ι' : ([], EApp v1 l0, []) |||| ι2 : p' |||| Π) with
             (ι1 : p'1 |||| ι' : ([], EApp v1 l0, []) |||| ι2 : p' |||| Π).
-    rewrite EQ. apply nother; auto.
+    rewrite EQ. apply n_other; auto.
     clear EQ H1 H2 H0.
-    all: unfold par in *; extensionality x;
+    all: unfold par, update in *; extensionality x;
          apply equal_f with x in H7; apply equal_f with x in H15;
          do 2 break_match_goal; subst; auto; try congruence.
     - break_match_goal; auto. subst. congruence.
     - break_match_goal; auto. subst. congruence.
+  * inversion H1; subst.
+    1: intuition; try congruence; destruct H5; congruence.
+    inversion H0. subst.
+    assert ((ι1 : p |||| (Π0 -- ι2)) = 
+             ι1 : p |||| (Π  -- ι2)) as EQ. {
+      extensionality x. unfold par, update in *. break_match_goal; auto.
+      apply internal_keep with (x := x) in H0. simpl in H0.
+      break_match_goal; auto. auto.
+    }
+    replace (Π0 -- ι2) with
+            (ι1 : p |||| (Π0 -- ι2)).
+    replace (Π -- ι2) with
+            (ι1 : p' |||| (Π -- ι2)).
+    rewrite EQ. constructor; auto.
+    all: unfold par, update in *; extensionality x;
+     apply equal_f with x in H6; apply equal_f with x in H11;
+     do 2 break_match_goal; subst; auto; try congruence.
 Qed.
 
 Theorem delay_internal_same :
@@ -631,11 +719,11 @@ Proof.
                end
               else (ι : p |||| Π) ι0) with
              (ι : (fst (fst p), snd (fst p), snd p ++ [t]) |||| prs).
-    2: { extensionality x. unfold par in *. apply equal_f with x in H5.
+    2: { extensionality x. unfold par, update in *. apply equal_f with x in H5.
          break_match_goal; auto.
          destruct p, p; subst. inversion H10; subst; auto.
        }
-    apply nother. 2: now left.
+    apply n_other. 2: now left.
     inversion H10; subst.
     inversion H2; simpl; subst.
     - constructor; auto.
@@ -663,12 +751,12 @@ Proof.
       + eapply internals_trans.
         exists l, k. split; eauto.
         exists [(AInternal, ι)], 1. split. repeat constructor.
-        eapply ntrans; eauto. constructor.
+        eapply n_trans; eauto. constructor.
       + epose proof (delay_internal_same _ _ _ H _ _ D1 _ H1).
         epose proof (IHD H5 _ _ _ _ H0 D1).
         eapply internals_trans. 2: exact H3.
         exists [(AInternal, ι)], 1. split. repeat constructor.
-        eapply ntrans. exact H2. apply nrefl.
+        eapply n_trans. exact H2. apply n_refl.
     - apply not_eq_sym in n0.
       epose proof (D2 := step_chain _ _ _ _ H _ _ _ _ H1 n0).
       destruct D2 as [n4 D2].
@@ -676,7 +764,7 @@ Proof.
 
       eapply internals_trans. 2: exact H2.
       exists [(AInternal, ι)], 1. split. repeat constructor.
-      eapply ntrans. 2: apply nrefl.
+      eapply n_trans. 2: apply n_refl.
       clear IHD H5 D All H2 H0.
       now epose proof (diamond_derivations _ _ _ _ _ _ _ n0 H H1 D2).
   Unshelve.
@@ -748,7 +836,7 @@ Proof.
   * apply internalSteps_weak_bisim.
   * exists [(AInternal, 0); (AInternal, 0)], 2. split.
     - repeat constructor.
-    - eapply ntrans. do 3 constructor.
-      eapply ntrans. do 4 constructor.
-      simpl. apply nrefl.
+    - eapply n_trans. do 3 constructor.
+      eapply n_trans. do 4 constructor.
+      simpl. apply n_refl.
 Qed.
